cp

coq/denot/definitions.v
@@ -14,6 +14,10 @@
    the set is the complete denotation of the value/computation. (These
    elements should be consistent with eachother.)
 
+   We can approximate infinite sets by the finite type `fset A`. 
+   Right now, this type is isomorphic to list, and we need to modify the 
+   definitions so that they respect set equality.
+
    The denotation of both values and computations includes bottom: the
    denotation of an infinite loop. Therefore, some definitions include
    the predicate
@@ -33,9 +37,9 @@
    this definition. So I have used the types above, and have defined the
    Monad-like operations:
 
-      RET : P A -> P (Comp (list A))
+      RET : P A -> P (Comp (fset A))
 
-      BIND : (P (Comp (list A))) -> (P A -> P (Comp B)) -> P (Comp B)
+      BIND : (P (Comp (fset A))) -> (P A -> P (Comp B)) -> P (Comp B)
 
    I don't know which of the analogous monad laws these operators satisfy.
 
@@ -51,9 +55,9 @@
 
       LIST : list (P Value) -> P Value
 
-      Λ : (P Value -> P (Comp (list Value))) -> P Value     -- note function bodies are computations
+      Λ : (P Value -> P (Comp (fset Value))) -> P Value     -- note function bodies are computations
 
-      APPLY : P Value -> P Value -> P (Comp (list Value))
+      APPLY : P Value -> P Value -> P (Comp (fset Value))
 
    Environments. An `Env A` is an association list, associating each variable with an `A`. 
 
@@ -75,7 +79,7 @@
 
    Denotation functions (mutually defined):
 
-       denot     : tm -> Rho -> P (Comp (list Value))
+       denot     : tm -> Rho -> P (Comp (fset Value))
 
        denot_val : tm -> Rho -> P Value
 
@@ -89,31 +93,12 @@ Require Import Lia.
 
 Require Export lc.tactics.
 Require Import structures.Structures.
+Require Export structures.consistency.
 
 Import MonadNotation.
 Open Scope monad_scope.
 Import SetNotations.
 Local Open Scope set_scope.
-
-
-(* 
-   Infinite sets of Values:   P Value      (i.e. Value -> Prop)
-   Finite sets of Values:     fset Value   (i.e. list Value)
-
-*)
-
-(* ------------------------------------------------------- *)
-
-Definition RET {A} (x : P A) : P (Comp (fset A)) :=
-  fun z => match z with 
-          | c_multi (V :: nil) => (mem V ⊆ x) /\ nonempty_fset V
-          |  _ => False
-        end.
-
-Definition BIND {A B} (S : P (Comp (fset A))) (K : P A -> P (Comp B)) (t : Comp B) : Prop :=
-  exists (u : Comp (fset A)), exists (k : fset A -> Comp B), 
-    (u ∈ S) /\ t = bind u k /\ forall a, Comp_In a u -> K (mem a) (k a).
-
 
 (* ----------------------------------------------------------- *)
 
@@ -121,7 +106,7 @@ Inductive Value : Type :=
   (* natural number *)
   | v_nat : nat -> Value
 
-  (* one entry in a function's table *)
+  (* one entry in a function's table. *)
   | v_map : fset Value -> Comp (fset Value) -> Value
 
   (* trivial function value, evaluated to a value but never applied *)
@@ -130,6 +115,10 @@ Inductive Value : Type :=
   (* list/tuple of values *)
   | v_list : list Value -> Value.
 
+#[export] Hint Constructors Value : core.
+
+Infix "↦" := v_map (at level 85, right associativity).
+
 (* EXAMPLE
 
 Denotation of Identity function (\x.x):  
@@ -137,84 +126,12 @@ Denotation of Identity function (\x.x):
   any subset of 
 
  { vfun } `union` 
- { v_map [v_nat vi] (c_multi ([v_nat vi] :: nil))  | for any value vi } 
+ { {v_nat vi} ↦ c_multi ( {v_nat vi} :: nil) | for any value vi } 
 
  *)
 
-#[export] Hint Constructors Value : core.
 
-Infix "↦" := v_map (at level 85, right associativity).
-
-(* ------------ Consistent ------------------ *)
-
-Class Consistency (A : Type) : Type := 
-  { Consistent : A -> A -> Prop ;
-    Inconsistent : A -> A -> Prop ;
-  }.
-
-Section List.
-
-Context 
-  { A : Type }
-  { f : A -> A -> Prop }
-  { g : A -> A -> Prop }.
-
-Definition Consistent_list := List.Forall2 f.
-Definition Inconsistent_list := fun XS YS => 
-  length XS <> length YS \/ List.Exists2 g XS YS.
-
-End List.
-
-#[export] Instance Consistency_list { A : Type } `{ Consistency A } : Consistency (list A) := 
-  { Consistent := Consistent_list (f := Consistent) ;
-    Inconsistent := Inconsistent_list (g := Inconsistent) ;
-  }.
-
-Section FSet.
-
-Context 
-  { A : Type }
-  { f : A -> A -> Prop }
-  { g : A -> A -> Prop }.
-
-Definition Consistent_fset := fun '(FSet XS) '(FSet YS) => List.Forall2_any f XS YS.
-Definition Inconsistent_fset := fun '(FSet XS) '(FSet YS) => List.Exists2_any g XS YS.
-
-End FSet.
-
-#[export] Instance Consistency_fset { A : Type}  `{ Consistency A } : Consistency (fset A) := 
-  { Consistent := Consistent_fset (f := Consistent) ;
-    Inconsistent := Inconsistent_fset (g := Inconsistent) ;
-  }.
-
-Section Computations.
-
-Context 
-  { A : Type }
-  { f : A -> A -> Prop }
-  { g : A -> A -> Prop }.
-
-Inductive ConsistentComp  : Comp A -> Comp A -> Prop :=
-  | cc_wrong : ConsistentComp c_wrong c_wrong
-  | cc_multi : forall AS BS, 
-      List.Forall2 f AS BS ->
-      ConsistentComp (c_multi AS) (c_multi BS).
-
-Inductive InconsistentComp : Comp A -> Comp A -> Prop :=
-  | i_wrong_multi : forall AS, InconsistentComp c_wrong (c_multi AS)
-  | i_multi_wrong : forall AS, InconsistentComp (c_multi AS) c_wrong
-  | i_multi : forall AS BS, 
-      (length AS <> length BS \/ List.Exists2 g AS BS) -> 
-      InconsistentComp (c_multi AS) (c_multi BS).
-
-End Computations.
-
-#[export] Instance Consistency_Comp {A:Type} `{Consistency A} : Consistency (Comp A) := 
-  { Consistent := ConsistentComp (f:=Consistent) ; Inconsistent := InconsistentComp (g := Inconsistent) }.
-
-#[export] Hint Constructors ConsistentComp InconsistentComp : core.
-
-(* ------------------------------------------------- *)
+(* ------------ Consistency for Values ------------------ *)
 
 (* Consistent values: we model function values as a set of approximations
 
@@ -244,11 +161,9 @@ Inductive ConsistentValue : Value -> Value -> Prop :=
   | c_list : forall (XS YS : list Value), 
       Consistent_list (f := ConsistentValue) XS YS ->      
       ConsistentValue (v_list XS) (v_list YS)
-
   | c_fun  : ConsistentValue v_fun v_fun
   | c_fun1 : forall X r, ConsistentValue v_fun (X ↦ r)
   | c_fun2 : forall X r, ConsistentValue (X ↦ r) v_fun
-
   | c_map2 : forall X1 X2 r1 r2, 
       Inconsistent_fset_Value X1 X2 ->
       ConsistentValue (X1 ↦ r1) (X2 ↦ r2)
@@ -268,6 +183,10 @@ with InconsistentValue : Value -> Value -> Prop :=
       Consistent_fset_Value X1 X2 ->
       InconsistentComp (g := Inconsistent_fset_Value) r1 r2 -> 
       InconsistentValue (X1 ↦ r1) (X2 ↦ r2)
+
+(* This part of the definition breaks the fset abstraction, 
+   but I was unable to get this to pass the positivity checker 
+   otherwise.  *)
 with Consistent_fset_Value : fset Value -> fset Value -> Prop :=
   | c_fset : forall X1 X2, 
     Consistent_fset (f := ConsistentValue) (FSet X1) (FSet X2) -> 
@@ -278,24 +197,15 @@ with Inconsistent_fset_Value : fset Value -> fset Value -> Prop :=
     Inconsistent_fset_Value (FSet X1) (FSet X2).
 
 
-#[export] Hint Constructors ConsistentValue InconsistentValue Consistent_fset_Value Inconsistent_fset_Value v_head : core.
+#[export] Hint Constructors ConsistentValue InconsistentValue 
+  Consistent_fset_Value Inconsistent_fset_Value v_head : core.
 
-Instance Consistency_Value : Consistency Value :=
+#[export] Instance Consistency_Value : Consistency Value :=
   { Consistent := ConsistentValue ; Inconsistent := InconsistentValue }.
 
-(* Two sets are consistent if all of their elements 
-   are consistent. *)
-Definition ConsistentSets {A:Type} `{Consistency A} V1 V2 := 
-    forall x y, x ∈ V1 -> y ∈ V2 -> Consistent x y.
 
-Definition InconsistentSets {A:Type} `{Consistency A} V1 V2 := 
-  exists x, exists y, (x ∈ V1) /\ (y ∈ V2) /\ (Inconsistent x y).
+Definition ConsistentSet {A:Type} `{Consistency A} (V : P A) := Consistent V V.
 
-#[export] Instance Consistency_P {A:Type} `{Consistency A} : Consistency (P A) :=
-   { Consistent := ConsistentSets ; Inconsistent := InconsistentSets }.
-
-
-Definition ConsistentSet {A:Type} `{Consistency A} (V : P A) := ConsistentSets V V.
 
 
 (* ------------ Semantic Operators ------------------ *)
@@ -318,7 +228,7 @@ Definition NIL : P Value := ⌈ v_list nil ⌉.
 Definition CONS : P Value -> P Value -> P Value := 
   fun V W x => 
     match x with 
-    | v_list (v :: w) => (v ∈ V) /\ (v_list w ∈ W)  (* v should not be wrong *)
+    | v_list (v :: w) => (v ∈ V) /\ (v_list w ∈ W)  
     | _ => False
     end.
 
@@ -345,13 +255,11 @@ Definition Λ : (P Value -> P (Comp (fset Value))) -> P Value :=
            << should this be empty or wrong??? >> 
 
    When does APPLY propagate wrong?
-    - wrong in D1 or D2  (FUNWRONG / ARGWRONG) 
     - V ↦ wrong in D1 and valid V in D2  (BETA case)
 
    When does APPLY create a new wrong? 
     - D1 contains a successful Value that is not a v_fun, v_map or v_list  (APPWRONG)
     - D1 contains a v_list and D2 contains a successful Value that is not a nat (PROJWRONG)
-           
 *)
 
 Inductive applicable : Value -> Prop :=
@@ -363,13 +271,14 @@ Inductive applicable : Value -> Prop :=
 
 Inductive APPLY : P Value -> P Value -> (Comp (fset Value) -> Prop) :=
   | BETA : forall D1 D2 w V,
-      (V ↦ w) ∈ D1 ->
+     (V ↦ w) ∈ D1 ->
      (mem V ⊆ D2) -> valid_mem V ->
      APPLY D1 D2 w
 
-(* NOTE: this definition is wrong! need to incorporate eta-expansion here to order for exists
+(* NOTE: this definition for PROJ is wrong! need to incorporate eta-expansion here
+   after we get the semantics of unification, choice, and sequencing down.
 
-  <v1 ... vn > i == (i=0;v1) | .. | (i=n;vn)
+       <v1 ... vn > i == (i=0;v1) | .. | (i=n;vn)
 
 *)
  
@@ -391,23 +300,26 @@ Infix "▩" := APPLY (at level 90).
 
 #[export] Hint Constructors APPLY : core.
 
+(* --------------- ADDITION ----------------------- *)
+
 Definition ADD : P Value :=
   fun w => 
     match w with 
     | (V ↦ c_multi (K :: nil)) => 
-        exists i j k, (mem V ≃ ⌈ v_list (v_nat i :: v_nat j :: nil) ⌉) /\ (mem K ≃ ⌈ v_nat k ⌉) /\ (k = i + j)
+        exists i j k, 
+        (mem V ≃ ⌈ v_list (v_nat i :: v_nat j :: nil) ⌉) /\ 
+        (mem K ≃ ⌈ v_nat k ⌉) /\ 
+        (k = i + j)
     | V ↦ c_wrong => 
         not (exists i j, v_list (v_nat i :: v_nat j :: nil) ∈ mem V) /\ valid_mem V
     | _ => False
     end.
 
-
-
 (* ------------ LOGIC PROGRAMMING ----------------- *)
 
 
 Definition ONE (C : P (Comp (fset Value))) : P Value :=
-  fun v => exists l, c_multi (singleton_fset v  :: l) ∈ C.
+  fun v => exists l, c_multi (singleton_fset v :: l) ∈ C.
 
 Definition ALL (C : P (Comp (fset Value))) : P Value :=
   fun v => match v with 
@@ -426,32 +338,68 @@ Definition CHOICE (C1 : P (Comp (fset Value))) (C2 : P (Comp (fset Value))) :
     | _ => False
     end.
 
-Definition SEQ (C1 : P (Comp (fset Value))) (C2 : P (Comp (fset Value))) : 
-  P (Comp (fset Value)) := BIND C1 (fun x => C2).
-
-(* Fails when V and W don't unify. Returns their union when they do. *)
-(* Can we replace last line below with "Consistent sets"? *)
+(* Fails when V and W don't unify. Returns an approximation of their union when they do. *)
 
 Definition UNIFY (V : P Value) (W: P Value) : P (Comp (fset Value)) :=
   fun c => match c with 
 
-        | c_multi nil => Inconsistent V W
+        | c_multi nil => 
+            Inconsistent V W
 
         | c_multi (l :: nil) => 
             exists l1, exists l2, l = union_fset l1 l2 /\ nonempty_fset l1 /\  nonempty_fset l2 
            /\ (mem l1 ⊆ V) /\ (mem l2 ⊆ W)
            /\ Consistent l1 l2
 
+        (* Could this instead read (this is a bit stronger than the above, but still strict?):
+
+           Consistent V W /\ mem l ⊆ (V ∪ W) /\ nonempty V /\ nonempty W
+
+         *)
+
         | _ => False
   end.
     
-(* Questions: Do we make sure the existentially chosen value is consisten? 
-   What about the final set? (Can we do that elsewhere?)
+(* Questions: 
+   Should we make sure the existentially chosen value is consistent? nonempty?
+   How do we think about the interaction between CHOICE and EXISTS?
 *)
 
 Definition EXISTS (f : P Value -> P (Comp (fset Value))) : P (Comp (fset Value)) :=
   fun c => exists V, c ∈ f (mem V).
 
+
+(* ------------------------------------------------------- *)
+
+(* 'Monadic operators' *)
+
+Definition RET {A} (x : P A) : P (Comp (fset A)) :=
+  fun z => match z with 
+          | c_multi (V :: nil) => (mem V ⊆ x) /\ nonempty_fset V
+          |  _ => False
+        end.
+
+(* NOTE: this is an alternative definition of RET, in terms of ret,
+   for the Comp type, and is more similar to the definition of 
+   BIND below. 
+
+Definition LIFT0 {A} (F : P A) : P (Comp (fset A)) :=
+  fun t =>  exists f : fset A, 
+      nonempty_fset f  /\ t = ret f /\ (mem f ⊆ F). 
+*)
+
+
+Definition BIND {A B} (S : P (Comp (fset A))) (K : P A -> P (Comp B)) (t : Comp B) : Prop :=
+  exists (u : Comp (fset A)), exists (k : fset A -> Comp B), 
+    (u ∈ S) /\ t = bind u k /\ forall a, Comp_In a u -> K (mem a) (k a).
+
+(* What happens if there is an empty set in u? Can we guarantee that 
+   the semantic operators above will be called with nonempty sets? *)
+
+Definition SEQ (C1 : P (Comp (fset Value))) (C2 : P (Comp (fset Value))) : 
+  P (Comp (fset Value)) := BIND C1 (fun x => C2).
+
+(* or:  RET (fun x y => y) <*> C1 <*> C2 *)
 
 (* ------------------------------------------------------- *)
 
@@ -507,39 +455,6 @@ Definition same_env : Rho -> Rho -> Prop := Env.Forall2 Same_set.
 Import LCNotations.
 Open Scope tm.
 
-Fixpoint exn (n : nat) (t: tm) : tm :=
-  match n with 
-  | 0 => t
-  | S n => ex (exn n t)
-  end.
-
-Fixpoint choice_free (t : tm) : bool :=
-  match t with 
-  | choice t u => false
-  | seq t u => choice_free t && choice_free u 
-  | unify t u => choice_free t && choice_free u 
-  | ex u => choice_free u
-  | _ => true
-  end.
-
-Inductive CX := CX_hole | CX_seq1 of tm | CX_seq2 of tm | CX_unify1 of tm | CX_unify2 of tm | CX_ex of tm.
-
-(* CX := [] | v = CX ; e | CX ; e | ceq ; CX | exists x. CX *)
-
-(*  CX [ e1 || e2 ] =>  CX [e1] || CX [e2] *)
-
-(* Pull out inner choice expressions, in order *)
-(* 
-Fixpoint choose  (s : tm) : CX * list tm :=
-  match s with 
-  | choice t u => CX_hole , t :: u :: nil
-  | seq t u => 
-  | unify t u => 
-  | ex t =>
-  | _ => s 
-  end *)
-
-
 (* Denotation function *)
 (* `n` is is a termination metric. *)
 Fixpoint denot_comp_n (n : nat) (a : tm) (ρ : Rho) : P (Comp (fset Value)) :=
@@ -573,25 +488,25 @@ Fixpoint denot_comp_n (n : nat) (a : tm) (ρ : Rho) : P (Comp (fset Value)) :=
       match a with 
        | app t u   => 
            BIND (denot_comp_n m t ρ) (fun v1 =>
-             BIND (denot_comp_n m u ρ) (fun v2 =>
-             (v1 ▩ v2))) 
+           BIND (denot_comp_n m u ρ) (fun v2 =>
+           (v1 ▩ v2))) 
 
        | tcons t u => 
-(*           RET CONS <*> (denot_comp_n m t ρ) <*> (denot_comp_n m u ρ) *)
-
            BIND (denot_comp_n m t ρ) (fun v1 =>
            BIND (denot_comp_n m u ρ) (fun v2 => 
            RET (CONS v1 v2 ))) 
 
-       | fail => FAIL
+       | fail => 
+           FAIL
 
-       | choice t u => CHOICE (denot_comp_n m t ρ) (denot_comp_n m u ρ)
+       | choice t u => 
+           CHOICE (denot_comp_n m t ρ) (denot_comp_n m u ρ)
 
-       | ex t => let x := fresh_for (dom ρ \u fv_tm t) in 
-                EXISTS (fun D => (denot_comp_n m (t ^ x) (x ~ D ++ ρ)))
+       | ex t => 
+           let x := fresh_for (dom ρ \u fv_tm t) in 
+           EXISTS (fun D => (denot_comp_n m (t ^ x) (x ~ D ++ ρ)))
 
-       | seq t u =>   
-           SEQ (denot_comp_n m t ρ) (denot_comp_n m u ρ)
+       | seq t u => SEQ (denot_comp_n m t ρ) (denot_comp_n m u ρ)
 
        | unify t u =>  
            BIND (denot_comp_n m t ρ) (fun v1 =>
@@ -637,4 +552,42 @@ Definition denot_val (a : tm) := denot_val_n (size_tm a) a.
 
 #[export] Hint Opaque denot : core.
 #[export] Hint Opaque denot_val : core.
+
+
+
+
+Fixpoint exn (n : nat) (t: tm) : tm :=
+  match n with 
+  | 0 => t
+  | S n => ex (exn n t)
+  end.
+
+Fixpoint choice_free (t : tm) : bool :=
+  match t with 
+  | choice t u => false
+  | seq t u => choice_free t && choice_free u 
+  | unify t u => choice_free t && choice_free u 
+  | ex u => choice_free u
+  | _ => true
+  end.
+
+(* Choice contexts *)
+Inductive CX := CX_hole | CX_seq1 of tm | CX_seq2 of tm | CX_unify1 of tm | CX_unify2 of tm | CX_ex of tm.
+
+(* CX := [] | v = CX ; e | CX ; e | ceq ; CX | exists x. CX *)
+
+(*  CX [ e1 || e2 ] =>  CX [e1] || CX [e2] *)
+
+(* Pull out inner choice expressions, in order *)
+(* 
+Fixpoint choose  (s : tm) : CX * list tm :=
+  match s with 
+  | choice t u => CX_hole , t :: u :: nil
+  | seq t u => 
+  | unify t u => 
+  | ex t =>
+  | _ => s 
+  end *)
+
+
 
